examples/steel/arraystructs/PointStruct.fst
@@ -65,8 +65,8 @@ let addr_of_x #a #x #y p =
   A.change_equal_slprop (q `pts_to` _) (q `pts_to` x);
   A.return q
 
-let un_addr_of_x #a #x #y p q =
-  un_addr_of_lens q p _x (mk_point none y) x;
+let unaddr_of_x #a #x #y p q =
+  unaddr_of_lens q p _x (mk_point none y) x;
   A.change_equal_slprop (p `pts_to` _) (p `pts_to` _)
 
 let addr_of_y #a #x #y p =
@@ -75,6 +75,6 @@ let addr_of_y #a #x #y p =
   A.change_equal_slprop (q `pts_to` _) (q `pts_to` y);
   A.return q
 
-let un_addr_of_y #a #x #y p q =
-  un_addr_of_lens q p _y (mk_point x none) y;
+let unaddr_of_y #a #x #y p q =
+  unaddr_of_lens q p _y (mk_point x none) y;
   A.change_equal_slprop (p `pts_to` _) (p `pts_to` _)
